rocq-skylabs-brick/theories/lang/cpp/semantics/genv.v
@@ -47,9 +47,17 @@ Record genv : Type :=
 { genv_tu : translation_unit
   (* ^ Implementation detail: the result of merging all the [translation_unit]s
   in the program. Might be replaced when fixing FM-2738. *)
+; genv_tu_canonical : TU.canonical genv_tu = genv_tu
+  (* ^ Linking produces a location-free translation unit.  Recording that
+     invariant lets public semantic relations use [TU.canonical] while
+     operational lookups keep using the linked unit directly. *)
 }.
 
 Existing Class genv.
+
+Definition genv_view (g : genv) : SemanticTU.t :=
+  SemanticTU.of_canonical g.(genv_tu).
+
 Definition genv_abi (g : genv) : abi.t :=
   g.(genv_tu).(abi).
 Definition pointer_size_bitsize (g : genv) : bitsize :=
@@ -62,7 +70,7 @@ Definition genv_byte_order (g : genv) : endian :=
   (genv_abi g).(abi.byte_order).
 Definition pointer_size (g : genv) := bitsize.bytesN (pointer_size_bitsize g).
 Definition genv_type_table (g : genv) : type_table :=
-  g.(genv_tu).(types).
+  SemanticTU.types (genv_view g).
 
 Definition signedness_of_char (σ : genv) (ct : char_type) : signed :=
   abi.signedness_of_char (genv_abi σ) ct.
@@ -77,7 +85,7 @@ Definition equivalent_int_type (g : genv) (ct : char_type) : integral_type.t :=
 
 (** [genv_leq a b] states that [b] is an extension of [a] *)
 Record genv_leq {l r : genv} : Prop :=
-{ tu_le : sub_module l.(genv_tu) r.(genv_tu) }.
+{ tu_le : view_sub_module (genv_view l) (genv_view r) }.
 Arguments genv_leq _ _ : clear implicits.
 
 #[global] Instance PreOrder_genv_leq : PreOrder genv_leq.
@@ -92,15 +100,24 @@ Definition genv_eq (l r : genv) : Prop :=
   genv_leq l r /\ genv_leq r l.
 
 #[global] Instance genv_tu_proper : Proper (genv_leq ==> sub_module) genv_tu.
-Proof. solve_proper. Qed.
-#[global] Instance genv_tu_flip_proper : Proper (flip genv_leq ==> flip sub_module) genv_tu.
-Proof. solve_proper. Qed.
+Proof. intros ?? [H]. exact H. Qed.
+#[global] Instance genv_tu_flip_proper :
+    Proper (flip genv_leq ==> flip sub_module) genv_tu.
+Proof. intros ?? [H]. exact H. Qed.
 
 (* Sadly, neither instance is picked up by [f_equiv]. *)
 #[global] Instance genv_abi_proper : Proper (genv_leq ==> eq) genv_abi.
-Proof. intros ?? []. rewrite /genv_abi. by apply abi_compat. Qed.
+Proof.
+  intros l r [H].
+  unfold view_sub_module, genv_view, SemanticTU.of_canonical in H.
+  apply abi_compat in H. exact H.
+Qed.
 #[global] Instance genv_abi_flip_proper : Proper (flip genv_leq ==> eq) genv_abi.
-Proof. intros ?? []. rewrite /genv_abi. by symmetry; apply abi_compat. Qed.
+Proof.
+  intros l r [H].
+  unfold view_sub_module, genv_view, SemanticTU.of_canonical in H.
+  symmetry. apply abi_compat in H. exact H.
+Qed.
 #[global] Instance pointer_size_bitsize_proper : Proper (genv_leq ==> eq) pointer_size_bitsize.
 Proof. intros ?? Hle. by rewrite /pointer_size_bitsize (genv_abi_proper _ _ Hle). Qed.
 #[global] Instance pointer_size_bitsize_flip_proper : Proper (flip genv_leq ==> eq) pointer_size_bitsize.
@@ -119,35 +136,82 @@ Proof. intros ?? Hle. by rewrite /genv_byte_order (genv_abi_flip_proper _ _ Hle)
  * compilation unit and that the [genv] contains addresses for all globals
  * defined in the [translation_unit]
  *)
+(** Semantic consumers ignore source-location wrappers while generated
+    translation units retain them for diagnostics and tooling. *)
 Class genv_compat {tu : translation_unit} {g : genv} : Prop :=
-{ tu_compat : sub_module tu g.(genv_tu) }.
+  Build_semantic_genv_compat
+  { tu_compat : view_sub_module (SemanticTU.of_tu tu) (genv_view g) }.
 Arguments genv_compat _ _ : clear implicits.
 Infix "⊧" := genv_compat (at level 1).
 
-Theorem genv_byte_order_tu tu g :
-    tu ⊧ g ->
-    genv_byte_order g = byte_order tu.
-Proof. intros. apply byte_order_flip_proper, tu_compat. Qed.
+(** Byte-order compatibility is weaker than full semantic compatibility.
+    Its legacy constructor name preserves the long-standing proof pattern
+    [apply Build_genv_compat; reflexivity] for the linked TU itself. *)
+Class genv_abi_compat (tu : translation_unit) (g : genv) : Prop :=
+  Build_genv_abi_compat
+  { genv_byte_order_compat : genv_byte_order g = byte_order tu }.
 
-Theorem genv_compat_submodule : forall m σ, m ⊧ σ -> sub_module m σ.(genv_tu).
+(** A legacy constructor name for proofs that only need byte-order
+    compatibility.  Keeping this as a definition, rather than as the class
+    constructor, prevents [eauto] from inventing an unrelated translation
+    unit when a semantic compatibility witness is already in scope. *)
+Definition Build_genv_compat tu g
+    (H : genv_byte_order g = byte_order tu) : genv_abi_compat tu g.
+Proof. by constructor. Defined.
+
+#[global] Instance genv_compat_abi tu g :
+    genv_compat tu g -> genv_abi_compat tu g.
+Proof.
+  move=>[H]. constructor.
+  apply byte_order_flip_proper in H. exact H.
+Qed.
+#[global] Hint Resolve genv_compat_abi : core.
+
+Theorem genv_byte_order_tu tu g :
+    genv_abi_compat tu g ->
+    genv_byte_order g = byte_order tu.
 Proof. by destruct 1. Qed.
 
-#[global] Instance genv_compat_proper : Proper (flip sub_module ==> genv_leq ==> impl) genv_compat.
+Theorem genv_compat_submodule : forall m σ, m ⊧ σ ->
+  sub_module (TU.canonical m) σ.(genv_tu).
+Proof. by destruct 1. Qed.
+
+Theorem genv_compat_semantic_submodule : forall m σ, m ⊧ σ ->
+  semantic_sub_module m σ.(genv_tu).
 Proof.
-  intros ?? Heq1 ?? [Heq2] [Heq3]; constructor.
-  by rewrite Heq1 Heq3.
+  intros m σ Hcompat.
+  rewrite semantic_sub_module_eq. unfold view_sub_module.
+  change (sub_module (TU.canonical m) (TU.canonical σ.(genv_tu))).
+  rewrite σ.(genv_tu_canonical).
+  exact (genv_compat_submodule m σ Hcompat).
 Qed.
-#[global] Instance genv_compat_flip_proper : Proper (sub_module ==> flip genv_leq ==> flip impl) genv_compat.
-Proof. solve_proper. Qed.
+#[global] Hint Resolve genv_compat_semantic_submodule : core.
+
+#[global] Instance genv_compat_proper :
+    Proper (flip semantic_sub_module ==> genv_leq ==> impl) genv_compat.
+Proof.
+  intros tu1 tu2 Htu g1 g2 [Hg] [Hcompat]. constructor.
+  try rewrite semantic_sub_module_eq in Htu.
+  etransitivity; [exact Htu|].
+  etransitivity; [exact Hcompat|exact Hg].
+Qed.
+#[global] Instance genv_compat_flip_proper :
+    Proper (semantic_sub_module ==> flip genv_leq ==> flip impl) genv_compat.
+Proof.
+  intros tu1 tu2 Htu g1 g2 [Hg] [Hcompat]. constructor.
+  try rewrite semantic_sub_module_eq in Htu.
+  etransitivity; [exact Htu|].
+  etransitivity; [exact Hcompat|exact Hg].
+Qed.
 
 Lemma module_le_genv_tu_models X σ :
-  module_le X (genv_tu σ) ->
+  view_module_le (SemanticTU.of_tu X) (genv_view σ) ->
   X ⊧ σ.
 Proof.
-  generalize (module_le_sound X (genv_tu σ)).
-  unfold Is_true in *.
-  case_match; try contradiction. intros.
-  apply Build_genv_compat. assumption.
+  move=> Hle. apply Build_semantic_genv_compat.
+  have Hspec := view_module_le_spec (SemanticTU.of_tu X) (genv_view σ).
+  case E: view_module_le in Hle; last contradiction.
+  rewrite E in Hspec. by inversion Hspec.
 Qed.
 
 (** ** One Definition Rule
@@ -164,20 +228,24 @@ Qed.
 Lemma ODR {σ tu1 tu2} :
     tu1 ⊧ σ ->
     tu2 ⊧ σ -> forall nm gd1 gd2,
-        tu1.(types) !! nm = Some gd1 ->
-        tu2.(types) !! nm = Some gd2 ->
+        SemanticTU.lookup_type (SemanticTU.of_tu tu1) nm = Some gd1 ->
+        SemanticTU.lookup_type (SemanticTU.of_tu tu2) nm = Some gd2 ->
         GlobDecl_compat gd1 gd2.
 Proof.
   move => [Hsub1] [Hsub2] nm gd1 gd2 H1 H2.
-  apply Hsub1 in H1 as [gd1' [Hlookup1 H1]].
-  apply Hsub2 in H2 as [gd2' [Hlookup2 H2]].
+  have H1' := eq_trans
+    (SemanticTU.lookup_type_spec (SemanticTU.of_tu tu1) nm) H1.
+  have H2' := eq_trans
+    (SemanticTU.lookup_type_spec (SemanticTU.of_tu tu2) nm) H2.
+  apply Hsub1 in H1' as [gd1' [Hlookup1 H1']].
+  apply Hsub2 in H2' as [gd2' [Hlookup2 H2']].
   rewrite Hlookup1 in Hlookup2. simplify_eq.
   by eapply GlobDecl_ler_join.
 Qed.
 
 (** TODO deprecate this in favor of inlining it *)
 Definition glob_def (σ : genv) (gn : name) : option GlobDecl :=
-  σ.(genv_tu).(types) !! gn.
+  genv_type_table σ !! gn.
 
 (*
 Lemma glob_def_alt σ gn :
@@ -187,27 +255,56 @@ Proof. done. Qed.
 
 (* Supersedes glob_def_submodule *)
 Lemma glob_def_genv_compat_struct {σ gn tu} {Hσ : tu ⊧ σ} st
-  (Hl : tu.(types) !! gn = Some (Gstruct st)) :
+  (Hl : SemanticTU.lookup_type (SemanticTU.of_tu tu) gn = Some (Gstruct st)) :
   glob_def σ gn = Some (Gstruct st).
-Proof. move: Hσ Hl => /genv_compat_submodule. apply: sub_module_preserves_gstruct. Qed.
+Proof.
+  have Hl' := eq_trans
+    (SemanticTU.lookup_type_spec (SemanticTU.of_tu tu) gn) Hl.
+  move: Hσ => /genv_compat_submodule Hsub.
+  unfold view_sub_module in Hsub.
+  unfold glob_def, genv_type_table, SemanticTU.types in *.
+  exact: sub_module_preserves_gstruct Hsub Hl'.
+Qed.
 
 Lemma glob_def_genv_compat_union {σ gn tu} {Hσ : tu ⊧ σ} st
-  (Hl : tu.(types) !! gn = Some (Gunion st)) :
+  (Hl : SemanticTU.lookup_type (SemanticTU.of_tu tu) gn = Some (Gunion st)) :
   glob_def σ gn = Some (Gunion st).
-Proof. move: Hσ Hl => /genv_compat_submodule. apply: sub_module_preserves_gunion. Qed.
+Proof.
+  have Hl' := eq_trans
+    (SemanticTU.lookup_type_spec (SemanticTU.of_tu tu) gn) Hl.
+  move: Hσ => /genv_compat_submodule Hsub.
+  unfold view_sub_module in Hsub.
+  unfold glob_def, genv_type_table, SemanticTU.types in *.
+  exact: sub_module_preserves_gunion Hsub Hl'.
+Qed.
 
 Lemma glob_def_genv_compat_enum {σ gn tu} {Hσ : tu ⊧ σ} ty brs
-  (Hl : tu.(types) !! gn = Some (Genum ty brs)) :
+  (Hl : SemanticTU.lookup_type (SemanticTU.of_tu tu) gn = Some (Genum ty brs)) :
   exists brs', glob_def σ gn = Some (Genum ty brs').
-Proof. move: Hσ Hl => /genv_compat_submodule. apply: sub_module_preserves_genum. Qed.
+Proof.
+  have Hl' := eq_trans
+    (SemanticTU.lookup_type_spec (SemanticTU.of_tu tu) gn) Hl.
+  move: Hσ => /genv_compat_submodule Hsub.
+  unfold view_sub_module in Hsub.
+  unfold glob_def, genv_type_table, SemanticTU.types in *.
+  exact: sub_module_preserves_genum Hsub Hl'.
+Qed.
 
 Lemma glob_def_genv_compat_constant {σ gn tu} {Hσ : tu ⊧ σ} ty e
-  (Hl : tu.(types) !! gn = Some (Gconstant ty (Some e))) :
+  (Hl : SemanticTU.lookup_type (SemanticTU.of_tu tu) gn = Some (Gconstant ty (Some e))) :
   glob_def σ gn = Some (Gconstant ty (Some e)).
-Proof. move: Hσ Hl => /genv_compat_submodule. apply: sub_module_preserves_gconstant. Qed.
+Proof.
+  have Hl' := eq_trans
+    (SemanticTU.lookup_type_spec (SemanticTU.of_tu tu) gn) Hl.
+  move: Hσ => /genv_compat_submodule Hsub.
+  unfold view_sub_module in Hsub.
+  unfold glob_def, genv_type_table, SemanticTU.types in *.
+  exact: sub_module_preserves_gconstant Hsub Hl'.
+Qed.
 
 (* XXX rename/deprecate? *)
-Theorem subModuleModels a b σ : b ⊧ σ -> sub_module a b -> a ⊧ σ.
+Theorem subModuleModels a b σ :
+    b ⊧ σ -> semantic_sub_module a b -> a ⊧ σ.
 Proof. by intros ? ->. Qed.
 
 (* TODO: [type_of_field] -- only needed in one place?
