rocq-skylabs-brick/theories/lang/cpp/syntax.v
@@ -9,7 +9,8 @@ Require Export skylabs.prelude.bytestring.
 Require Export skylabs.lang.cpp.syntax.preliminary.	(* syntax/preliminary.v *)
 Require Export skylabs.lang.cpp.syntax.overloadable.	(* syntax/overloadable.v *)
 Require Export skylabs.lang.cpp.syntax.core.	(* syntax/core.v *)
-Require Export skylabs.lang.cpp.syntax.loc_info.	(* syntax/loc_info.v *)
+Require skylabs.lang.cpp.syntax.loc_info.	(* syntax/loc_info.v *)
+Module LocInfo := skylabs.lang.cpp.syntax.loc_info.LocInfo.
 Require Export skylabs.lang.cpp.syntax.types.	(* syntax/types.v *)
 Require Export skylabs.lang.cpp.syntax.typing.	(* syntax/typing.v *)
 Require Export skylabs.lang.cpp.syntax.stmt.	(* syntax/stmt.v *)
